lca is now properly defined

history.fst
@@ -49,84 +49,98 @@ and size' l =
   | [] -> 0
   | x::xs -> size x + size' xs
 
-val lemma1: #n: nat -> h:history n{wellformed h} 
-          -> Lemma (ensures (forall c1 c2. mem c1 h /\ mem c2 h ==> length c1 = length c2)) (decreases (size h))
-let rec lemma1 h = 
-  let History c s ch = h in
+val lemma1 : #n:nat -> h:history n{wellformed h}
+           -> Lemma (ensures (forall h'. L.mem h' (History?.children h) ==> wellformed h')) (decreases (size h))
+let rec lemma1 (History c s ch) =
   match ch with
   | [] -> ()
-  | x::xs -> lemma1 (History c s xs); lemma1 x
+  | x::xs -> assert (wellformed x); lemma1 (History c s xs)
 
 val lemma2 : #n:nat -> h:history n{wellformed h}
-           -> Lemma (ensures (forall h'. L.mem h' (History?.children h) ==> wellformed h')) (decreases (size h))
-let rec lemma2 (History c s ch) =
-  match ch with
-  | [] -> ()
-  | x::xs -> assert (wellformed x); lemma2 (History c s xs)
-
-val lemma3 : #n:nat -> h:history n{wellformed h}
-          -> Lemma (ensures (forall h'. L.mem h' (History?.children h) ==> Vc.hbeq (History?.clock h) (History?.clock h'))) (decreases (size h))
-let rec lemma3 (History c s ch) =
-  match ch with
-  | [] -> ()
-  | x::xs -> assert (wellformed x); lemma3 (History c s xs); lemma3 x
-
-val lemma4 : #n:nat -> h:history n{wellformed h}
            -> Lemma (ensures (forall c. mem c h ==> Vc.hbeq (History?.clock h) c)) (decreases (size h))
-val lemma5 : #n:nat -> h:history n{wellformed h} -> c:Vc.t n{Vc.hbeq c (History?.clock h)}
+val lemma2' : #n:nat -> h:history n{wellformed h} -> c:Vc.t n{Vc.hbeq c (History?.clock h)}
            -> Lemma (requires (forall k. mem k h ==> Vc.hbeq (History?.clock h) k))
                    (ensures  (forall k. mem k h ==> Vc.hbeq c k)) (decreases (size h))
-let rec lemma4 h =
+let rec lemma2 h =
   let History c s ch = h in
   match ch with
   | [] -> Vc.hbeq_reflexive c
   | x::xs ->
-      lemma4 x;
-      lemma4 (History c s xs);
+      lemma2 x;
+      lemma2 (History c s xs);
       assert (Vc.hbeq c (History?.clock x));
       assert (forall k. mem k x ==> Vc.hbeq (History?.clock x) k);
-      lemma5 x c;
+      lemma2' x c;
       assert (forall k. mem k x ==> Vc.hbeq c k);
       ()
-and lemma5 (History c' s ch) c =
+and lemma2' (History c' s ch) c =
   match ch with
   | [] -> ()
   | x::xs -> 
       Vc.hbeq_transitive (length c) c c' (History?.clock x);
-      lemma4 x;
-      lemma5 x c;
-      lemma4 (History c' s xs);
-      lemma5 (History c' s xs) c;
+      lemma2 x;
+      lemma2' x c;
+      lemma2 (History c' s xs);
+      lemma2' (History c' s xs) c;
       ()
 
-val lca_ : #n:nat 
-        -> h:history n{wellformed h}
-        -> a:Vc.t n 
-        -> b:Vc.t n 
-        -> init:Vc.t n{Vc.hbeq init a /\ Vc.hbeq init b}
-        -> Tot (r:Vc.t n{Vc.hbeq r a /\ Vc.hbeq r b}) (decreases %[h])
-val lca_' : #n:nat 
-         -> l:list (history n){forall h. L.mem h l ==> wellformed h} 
-         -> a:Vc.t n 
-         -> b:Vc.t n 
-         -> init:Vc.t n{Vc.hbeq init a /\ Vc.hbeq init b}
-         -> Tot (r:Vc.t n{Vc.hbeq r a /\ Vc.hbeq r b}) (decreases %[l])
-let rec lca_ h a b init =
-  lemma2 h;
-  let History clock _ ch = h in
-  if Vc.hbeq init clock && Vc.hbeq clock a && Vc.hbeq clock b
-  then lca_' ch a b clock
-  else init
-and lca_' l a b init =
-  match l with
-  | [] -> init 
-  | x::xs -> lca_' xs a b (lca_ x a b init)
+val append : #n:nat -> p:(Vc.t n -> bool) 
+           -> l1:list (Vc.t n){forall e. L.mem e l1 ==> p e}
+           -> l2:list (Vc.t n){forall e. L.mem e l2 ==> p e}
+           -> l:list (Vc.t n){forall e. L.mem e l ==> p e}
+let rec append p l1 l2 =
+  match l1 with
+  | [] -> l2
+  | x::xs -> x::(append p xs l2)
 
-val lca : #n:nat
-       -> h:history n{wellformed h}
-       -> a:Vc.t n{mem a h}
-       -> b:Vc.t n{mem b h}
-       -> r:Vc.t n{Vc.hbeq r a /\ Vc.hbeq r b}
-let lca h a b = 
-  lemma4 h;
-  lca_ h a b (History?.clock h)
+val is_concurrent : #n:nat -> v:Vc.t n -> l:list (Vc.t n) 
+                  -> r:bool{(forall c. L.mem c l ==> (v = c \/ Vc.concurrent v c)) <==> r = true}
+let rec is_concurrent v l =
+  match l with
+  | [] -> true
+  | x::xs -> (v = x || Vc.concurrent v x) && is_concurrent v xs
+
+val cross_concurrent : #n:nat -> l:list (Vc.t n) 
+                     -> r:list (Vc.t n){(forall c. L.mem c r ==> L.mem c l) /\ 
+                                       (forall c1 c2. L.mem c1 r /\ L.mem c2 r ==> c1 = c2 \/ Vc.concurrent c1 c2)}
+let rec cross_concurrent l1 =
+  match l1 with
+  | [] -> []
+  | x::xs -> 
+      if is_concurrent x xs then begin
+        x::(cross_concurrent xs)
+      end else cross_concurrent xs 
+
+val get_latest : #n:nat -> p:(Vc.t n -> bool)
+               -> l:list (Vc.t n){forall c. L.mem c l ==> p c}
+               -> l':list (Vc.t n){(forall c. L.mem c l' ==> L.mem c l /\ p c)}
+let get_latest p l = cross_concurrent l
+
+val lca : #n:nat -> h:history n{wellformed h} -> a:Vc.t n{mem a h} -> b:Vc.t n{mem b h}
+        -> Tot (lcalst:list (Vc.t n){(forall l. L.mem l lcalst ==> mem l h /\ Vc.hbeq l a /\ Vc.hbeq l b) /\
+                                    (forall c1 c2. L.mem c1 lcalst /\ L.mem c2 lcalst ==> c1 = c2 \/ Vc.concurrent c1 c2)}) (decreases (size h))
+let rec lca h a b =
+  lemma2 h;
+  let History c s ch = h in
+  match ch with
+  | [] -> [c]
+  | x::xs ->
+      let l1 =
+        if mem a x && mem b x then
+            lca x a b
+        else []
+      in
+      let h' = History c s xs in
+      let l2 =
+        if mem a h' && mem b h' then
+            lca h' a b
+        else []
+      in
+      assert (forall c. L.mem c l1 ==> mem c h /\ Vc.hbeq c a /\ Vc.hbeq c b);
+      assert (forall c. L.mem c l2 ==> mem c h /\ Vc.hbeq c a /\ Vc.hbeq c b);
+      assert (mem c h /\ Vc.hbeq c a /\ Vc.hbeq c b);
+      let l = (c::(l1@l2)) in
+      let p = fun c -> mem c h && Vc.hbeq c a && Vc.hbeq c b in
+      let l = c::(append p l1 l2) in
+      assert (forall c. L.mem c l ==> mem c h /\ Vc.hbeq c a /\ Vc.hbeq c b);
+      get_latest p l
