vector_clock.fst
@@ -46,7 +46,7 @@ val hbeq_reflexive : #n:nat -> v:t n -> Lemma (ensures (hbeq v v))
 let hbeq_reflexive v = lemma1 v
 
 val lemma2 : v1:list nat -> v2:list nat{length v1 = length v2} 
-          -> Lemma (ensures (compare v1 v2 = Equal ==> v1 = v2))
+          -> Lemma (ensures (compare v1 v2 = Equal <==> v1 = v2))
 let rec lemma2 v1 v2 = 
   match v1, v2 with
   | [], [] -> ()
@@ -63,3 +63,71 @@ let rec hbeq_transitive n v1 v2 v3 =
        match v1, v2, v3 with
        | x::[], y::[], z::[] -> ()
        | x::xs, y::ys, z::zs -> hbeq_transitive (n - 1) xs ys zs
+
+val concurrent : #n:nat -> v1:t n -> v2:t n -> bool
+let concurrent v1 v2 = compare v1 v2 = Concurrent
+
+(*
+val lemma3 : x:nat -> xs:list nat -> y:nat{x < y} 
+           -> ys:list nat{length xs = length ys /\ compare xs ys = Happened_after} 
+           -> Lemma (ensures (compare (x::xs) (y::ys) = Concurrent))
+let lemma3 x xs y ys = ()
+
+val lemma4 : x:nat -> xs:list nat -> y:nat{x > y} 
+           -> ys:list nat{length xs = length ys /\ compare xs ys = Happened_before} 
+           -> Lemma (ensures (compare (x::xs) (y::ys) = Concurrent))
+let lemma4 x xs y ys = ()
+
+val lemma5 : x:nat -> xs:list nat -> y:nat{x > y}
+             -> ys:list nat{length xs = length ys /\ compare xs ys = Equal}
+             -> Lemma (ensures (compare (x::xs) (y::ys) = Happened_after))
+let lemma5 x xs y ys = ()
+
+val lemma6 : x:nat -> xs:list nat -> y:nat{x < y}
+             -> ys:list nat{length xs = length ys /\ compare xs ys = Equal}
+             -> Lemma (ensures (compare (x::xs) (y::ys) = Happened_before))
+let lemma6 x xs y ys = ()
+*)
+
+val lemma7 : n:nat -> v1:t n -> v2:t n{compare v1 v2 = Happened_after} 
+           -> Lemma (ensures (compare v2 v1 = Happened_before))
+let rec lemma7 n v1 v2 =
+  match v1, v2 with
+  | [], [] -> ()
+  | x::xs, y::ys -> 
+      if x = y then lemma7 (n-1) xs ys 
+      else if x < y then  ()
+      else match compare xs ys with
+           | Happened_after -> lemma7 (n-1) xs ys
+           | Equal -> lemma2 xs ys
+           | _ -> ()
+           
+val lemma8 : n:nat -> v1:t n -> v2:t n{compare v1 v2 = Happened_before} 
+           -> Lemma (ensures (compare v2 v1 = Happened_after))
+let rec lemma8 n v1 v2 =
+  match v1, v2 with
+  | [], [] -> ()
+  | x::xs, y::ys -> 
+      if x = y then lemma8 (n-1) xs ys 
+      else if x < y then
+        match compare xs ys with
+        | Happened_before -> lemma8 (n-1) xs ys
+        | Equal -> lemma2 xs ys
+        | _ -> ()
+      else () 
+
+val concurrent_commutative : n:nat -> v1:t n -> v2:t n{concurrent v1 v2}
+                           -> Lemma (ensures (concurrent v2 v1))
+                           [SMTPat (concurrent v1 v2)]
+let rec concurrent_commutative n v1 v2 =
+  match v1, v2 with
+  | [], [] -> ()
+  | x::xs, y::ys -> 
+      if x = y then concurrent_commutative (n-1) xs ys
+      else if x < y then
+        match compare xs ys with
+        | Concurrent -> concurrent_commutative (n-1) xs ys
+        | Happened_after -> lemma7 (n-1) xs ys
+      else match compare xs ys with
+           | Concurrent -> concurrent_commutative (n-1) xs ys
+           | Happened_before -> lemma8 (n-1) xs ys
